src/proof/algebra/kview.v
@@ -368,8 +368,8 @@ Proof.
     + subst k. rewrite /KObjectV.key /= Hobj_meta_eq //.
     + split.
       * rewrite Hobj_meta_eq in Huid_obj. symmetry. exact Huid_obj.
-      * apply valid_object_has_valid_objectmeta in Hwf_obj.
-        by rewrite Hobj_meta_eq in Hwf_obj.
+      * destruct obj; unfold KObjectV.valid in Hwf_obj; destruct Hwf_obj as (_ & Hwf_meta & _);
+        rewrite Hobj_meta_eq in Hwf_meta; done.
 Qed.
 
 Lemma auth_meta_valid a k uid dq meta:
