src/proof/kubernetes_model/common.v
@@ -1,17 +1,34 @@
 From New.proof Require Import prelude empty_ffi.
-From New.proof.kubernetes_model Require Export inv.
+From New.proof.kubernetes_model Require Export apimodel_init.
+From New.proof Require Export pure_objects.
 
 Section proof.
 Context `{hG: !heapGS Σ} {go_ctx: GoContext}.
 
-Lemma wp_deepCopy i pure_obj:
+Lemma wp_deepCopy i obj:
   {{{ is_pkg_init apimodel ∗
-      KObjectV.deepown_i i pure_obj 1
+      KObjectV.deepown_i i obj 1
   }}}
     @! apimodel.deepCopy #i
   {{{ i', RET #i';
-      KObjectV.deepown_i i' pure_obj 1 ∗
-      KObjectV.deepown_i i pure_obj 1
+      KObjectV.deepown_i i' obj 1 ∗
+      KObjectV.deepown_i i obj 1
+  }}}.
+Proof.
+Admitted.
+
+Lemma wp_applyValidationAndDefaulting i o (name : go_string):
+  {{{ is_pkg_init apimodel ∗
+      KObjectV.deepown_i i o 1 ∗
+      ⌜ ObjectMetaV.valid (KObjectV.objectmeta o) ⌝
+  }}}
+    @! apimodel.applyValidationAndDefaulting #i #name
+  {{{ o', RET #interface.nil;
+      KObjectV.deepown_i i o' 1 ∗
+      ⌜ ObjectMetaV.valid (KObjectV.objectmeta o') ⌝ ∗
+      ⌜ KObjectV.objectmeta o' = ((KObjectV.objectmeta o) <| ObjectMetaV.Generation' := W64 1 |>) ⌝ ∗
+      ⌜ ObjectSpecV.created (KObjectV.spec o) (KObjectV.spec o') ⌝ ∗
+      ⌜ ObjectStatusV.created (KObjectV.status o) (KObjectV.status o') ⌝
   }}}.
 Proof.
 Admitted.
